rr_frontend/translation/src/body/mod.rs
@@ -4,7 +4,5 @@
 // If a copy of the BSD-3-clause license was not distributed with this
 // file, You can obtain one at https://opensource.org/license/bsd-3-clause/.
 
-mod checked_op_analysis;
-
 pub mod signature;
 mod translation;
